Quicksort/Partition/BentleyMcIlroy/Basic.lean
@@ -1,0 +1,438 @@
+import Quicksort.Partition.Init.Basic
+
+private def dbg {α : Type u} [ToString α] (a : α) (s : String)  : α :=
+  dbgTrace s!"{s}" (fun _ => a)
+
+private instance [ToString α] : ToString (Vector α n) where
+  toString v := s!"#v{v.toList}"
+open Vector
+
+
+
+
+
+
+@[inline]
+def Partition.bentleyMcIlroy [Inhabited α] /- [ToString α] -/ [Ord α] {n : Nat}
+    (arr : Vector α n) (left : Nat)  (right : Nat) (hlr : left < right) (hr : right < n) :
+    {x : Partition α n // (left < x.i') ∧ (x.j' < right)} :=
+
+
+  let rec @[specialize] loop (pivot : α) (arr : Vector α n) (i j p q : Nat) : Vector α n × Nat × Nat × Nat × Nat :=
+    let rec @[specialize] findI (i : Nat) :=
+      -- i < n
+      have right := right
+      if /- i < right ∧ -/ lt arr[i]! pivot then
+        findI (i + 1)
+      else
+        i
+    termination_by right - i
+    decreasing_by sorry
+
+    let rec @[specialize] findJ (j : Nat) :=
+      -- 0 < j
+      if /- left < j ∧ -/ lt pivot arr[j]! then
+        findJ (j - 1)
+      else
+        j
+      termination_by j
+      decreasing_by sorry
+
+    let i' := findI (i + 1)
+    let j' := findJ (j - 1)
+
+    if i' < j' then Id.run do
+      let mut arr := arr.swap i' j' sorry sorry
+      let mut p := p
+      let mut q := q
+
+      -- if ¬ (lt arr[i]! pivot) ∧ ¬ (lt pivot arr[i]!) then
+      if ¬ lt arr[i']! pivot then
+        p := p + 1
+        arr := arr.swap p i' sorry sorry
+
+      -- if ¬ (lt arr[j]! pivot) ∧ ¬ (lt pivot arr[j]!) then
+      if ¬ lt pivot arr[j']! then
+        q := q - 1
+        arr := arr.swap q j' sorry sorry
+
+      loop pivot arr i' j' p q
+
+    else
+      (arr, i', j', p, q)
+    termination_by j + 1 - i
+    decreasing_by sorry
+
+
+  let mid := left + (right - left) / 2
+  let arr_ := arr
+    |> (Vector.maybeSwap . ⟨left, (by omega)⟩ ⟨right, (by omega)⟩)
+    |> (Vector.maybeSwap . ⟨mid, (by omega)⟩ ⟨right, (by omega)⟩)
+    |> (Vector.maybeSwap . ⟨mid, (by omega)⟩ ⟨left, (by omega)⟩)
+
+  -- let arr := arr.swap left mid (by omega) (by omega)
+  let pivot := arr_[left]
+
+
+  Id.run do
+    -- let mut (arr', i', j', p, q) := loop pivot arr_ left (right + 1) left (right + 1)
+    let mut (arr', i', j', p, q) := loop pivot arr_ left (right + 1) left (right + 1)
+
+    -- arr := arr.swap left j (sorry) (sorry)
+    -- j := j - 1
+
+    for k in [left : p + 1] do
+      arr' := arr'.swap k j' sorry sorry
+      j' := j' - 1
+
+
+    for k in [q : right + 1] do
+      arr' := arr'.swap k i' sorry sorry
+      i' := i' + 1
+
+    return ⟨⟨arr', j', i'⟩, by sorry, by sorry⟩
+
+
+
+
+
+
+
+#eval! Partition.bentleyMcIlroy #v[9,  3,  1,  8,  6,  2,  5,  0,  7,  4]  0 9 (by omega) (by omega)
+#eval! Partition.bentleyMcIlroy #v[9,  3,  1,  8,  6,  2,  6,  0,  7,  4]  0 9 (by omega) (by omega)
+#eval! Partition.bentleyMcIlroy #v[0, 2, 2, 1, 2]  0 4 (by omega) (by omega)
+
+
+
+
+
+
+
+
+
+
+
+
+
+
+
+
+
+
+
+
+
+
+
+
+
+
+
+
+
+
+-- @[inline]
+-- partial def Partition.bentleyMcIlroy [Inhabited α] /-  [BEq α] -/ [ToString α]
+--     [Ord α] {n : Nat}
+--     (arr : Vector α n) (left : Nat)  (right : Nat) (hlr : left < right) (hr : right < n) :
+--     {x : Partition α n // (left < x.i') ∧ (x.j' < right)} := Id.run do
+--     -- IO Unit := do
+--   let arr := dbg arr s!"arr : {arr}"
+
+--   let mid := left + (right - left) / 2
+--   let mut arr := arr
+--     |> (maybeSwap · ⟨left, sorry⟩ ⟨mid, sorry⟩)
+--     |> (maybeSwap · ⟨left, sorry⟩ ⟨right, sorry⟩)
+--     |> (maybeSwap · ⟨mid, sorry⟩ ⟨right, sorry⟩)
+
+
+--   arr := arr.swap left mid sorry sorry
+--   arr := dbg arr s!"arr_: {arr}"
+
+--   let pivot := arr[left]
+--   arr := dbg arr s!"pivot: {pivot}"
+
+
+--   let mut i := left
+--   let mut j := right + 1
+
+--   let mut p := left
+--   let mut q := right + 1
+
+-- -----------
+
+--   while true do
+--     i := i + 1
+--     while lt arr[i]! pivot do
+--       i := i + 1
+
+--     j := j - 1
+--     while lt pivot arr[j]! do
+--       j := j - 1
+
+--     if i ≥ j then
+--       break
+
+--     arr := arr.swap i j sorry sorry
+
+--     -- if arr[i] == pivot do
+--     if ¬ lt arr[i]! pivot then
+--       p := p + 1
+--       arr := arr.swap p i sorry sorry
+
+--     -- if arr[j] == pivot do
+--     if ¬ lt pivot arr[j]! then
+--       q := p + 1
+--       arr := arr.swap q j sorry sorry
+
+
+--   arr := arr.swap left j sorry sorry
+--   let mut j' := j - 1
+
+--   for k in [left + 1 : p + 1] do
+--       arr := arr.swap k j' sorry sorry
+--       j' := j' - 1
+
+--   let mut i' := i
+--   for k in [q : right + 1] do
+--       arr := arr.swap k i' sorry sorry
+--       i' := i' + 1
+
+
+
+--   return ⟨⟨arr, j', i'⟩, by sorry, by sorry⟩
+-- #eval! Partition.bentleyMcIlroy #v[9,  3,  1,  8,  6,  2,  5,  0,  7,  4]  0 9 (by omega) (by omega)
+
+
+
+-- #eval! Partition.bentleyMcIlroy #v[9,  3,  1,  8,  6,  2,  6,  0,  7,  4]  0 9 (by omega) (by omega)
+-- #eval! Partition.bentleyMcIlroy #v[0, 2, 2, 1, 2]  0 4 (by omega) (by omega)
+
+
+
+
+
+
+
+
+
+
+
+
+
+
+
+
+
+
+
+
+
+
+
+
+
+
+
+
+
+
+
+
+
+
+
+
+
+-- @[inline]
+-- partial def Partition.bentleyMcIlroy [Inhabited α] /-  [BEq α] -/ [ToString α]
+--     [Ord α] {n : Nat}
+--     (arr : Vector α n) (left : Nat)  (right : Nat) (hlr : left < right) (hr : right < n) :
+--     {x : Partition α n // (left < x.i') ∧ (x.j' < right)} := Id.run do
+--     -- IO Unit := do
+--   let mid := left + (right - left) / 2
+
+--   let arr := dbg arr s!"arr : {arr}"
+--   let mut arr := arr
+--     |> (maybeSwap · ⟨left, sorry⟩ ⟨mid, sorry⟩)
+--     |> (maybeSwap · ⟨left, sorry⟩ ⟨right, sorry⟩)
+--     |> (maybeSwap · ⟨mid, sorry⟩ ⟨right, sorry⟩)
+
+--   arr := dbg arr s!"arr_: {arr}"
+
+--   let pivot := arr[mid]!
+--   arr := dbg arr s!"pivot: {pivot}"
+
+--   let mut i := left + 1
+--   let mut j := right - 1
+
+--   let mut l := left + 1
+--   let mut r := right - 1
+
+--   arr := dbg arr s!"l:{l}, i:{i}   ---  {j}:j, {r}:r"
+--   let mut count := 0
+--   while count < 3 do
+
+--     while i < right ∧ lt arr[i]! pivot do
+--       i := i + 1
+--       -- if i == right then break
+
+--     while left < j ∧ lt pivot arr[j]! do
+--       j := j - 1
+--       -- if j == left then break
+
+
+--     if i ≥ j then --return
+--       arr := dbg arr s!"(j, i) := ({j}, {i})"
+--       break
+
+--     arr := dbg arr s!"arr1: {arr}, {i}, {j}"
+--     arr := arr.swap i j sorry sorry
+
+
+--     if ¬ lt arr[i]! pivot then
+--       arr := dbg arr s!"arri: {arr}, {i}, {l}"
+--       arr := arr.swap i l sorry sorry
+--       l := l + 1
+
+--     if ¬ lt pivot arr[j]! then
+--       arr := dbg arr s!"arrj: {arr}, {j}, {r}"
+--       arr := arr.swap j r sorry sorry
+--       r := r - 1
+
+--     count := count + 1
+--     count := dbg count s!"count := {count}"
+--   -- end while
+--   arr := dbg arr s!"(j, i) := ({j}, {i})"
+
+
+--   arr := dbg arr s!"left:  {left},  l: {l}"
+--   arr := dbg arr s!"right: {right},  r: {r}"
+
+--   -- arr := arr.swap left j sorry sorry
+--   arr := dbg arr s!"arr2: {arr}"
+--   -- -- i := i + 1
+--   -- j := j - 1
+--   for l_ in [left+1:l] do
+--     arr := dbg arr s!"larr: {arr}, {l_}, {j}"
+--     arr := arr.swap l_ j sorry sorry
+--     j := j - 1
+
+--   for r_ in [r+1:right] do
+--     arr := dbg arr s!"rarr: {arr}, {r_}, {i}"
+--     arr := arr.swap r_ i sorry sorry
+--     i := i + 1
+
+
+--   -- arr := dbg arr $ toString (arr, j, i)
+--   return ⟨⟨arr, j, i⟩, by sorry, by sorry⟩
+
+-- -- #eval! Partition.bentleyMcIlroy #v[9,  3,  1,  8,  6,  2,  5,  0,  7,  4]  0 9 (by omega) (by omega)
+
+
+
+-- -- #eval! Partition.bentleyMcIlroy #v[9,  3,  1,  8,  6,  2,  6,  0,  7,  4]  0 9 (by omega) (by omega)
+-- #eval! Partition.bentleyMcIlroy #v[0, 2, 2, 1, 2]  0 4 (by omega) (by omega)
+
+
+
+
+
+
+
+
+
+
+
+
+
+
+    -- if ¬lt arr[i]! pivot ∧ ¬lt pivot arr[i]! then
+    --   -- panic! "ERROR: arri == piv"
+    --   l := l + 1
+    --   arr := arr.swap i l sorry sorry
+
+    -- if ¬lt arr[j]! pivot ∧ ¬lt pivot arr[j]! then
+    --   -- panic! "ERROR: arrj == piv"
+    --   r := r - 1
+    --   arr := arr.swap j r sorry sorry
+
+
+
+
+
+
+
+
+
+-- @[inline]
+-- partial def Partition.bentleyMcIlroy [Inhabited α]  [Ord α] {n : Nat} (arr : Vector α n) (left : Nat)  (right : Nat) (hlr : left < right) (hr : right < n) : {x : Partition α n // (left < x.i') ∧ (x.j' < right)} :=
+
+--   -- let arr_ := arr
+--   --   |> (maybeSwap · ⟨left, by omega⟩ ⟨mid, by omega⟩)
+--   --   |> (maybeSwap · ⟨left, by omega⟩ ⟨right, by omega⟩)
+--   --   |> (maybeSwap · ⟨right, by omega⟩ ⟨mid, by omega⟩)
+--   -- have pivot := arr_[right]
+
+--   let mid := left + (right - left) / 2
+--   let arr' := arr
+--     |> (maybeSwap · ⟨left, sorry⟩ ⟨mid, sorry⟩)
+--     |> (maybeSwap · ⟨left, sorry⟩ ⟨right, sorry⟩)
+--     |> (maybeSwap · ⟨mid, sorry⟩ ⟨right, sorry⟩)
+--   let pivot := arr'[mid]!
+
+
+--   let rec  scan_i (a : Vector α n) (i : Nat) : Nat :=
+--     if i ≤ right ∧ lt a[i]! pivot then
+--       scan_i a (i + 1)
+--     else
+--       i
+
+--   let rec  scan_j (a : Vector α n) (j : Nat) : Nat :=
+--     if left ≤ j ∧ lt pivot a[j]! then
+--       scan_j a (j - 1)
+--     else
+--       j
+
+
+--   let rec main_loop (a : Vector α n) (i j p q : Nat) : Vector α n × Nat × Nat × Nat × Nat :=
+--     let i' := scan_i a (i + 1)
+--     let j' := scan_j a (j - 1)
+--     if i' < j' then
+--       let a' := a.swap i' j' sorry sorry
+--     -- ¬ lt a'[j']! pivot
+--     -- ¬ lt pivot a'[i']!
+--       let (a'', p') :=
+--         if lt pivot a'[i']! then
+--           (a', p)
+--         else
+--           (a'.swap (p + 1) i' sorry sorry, p + 1)
+--       let (a''', q') :=
+--         if lt a''[j']! pivot then
+--           (a'', q)
+--         else
+--           (a''.swap (q - 1) j' sorry sorry, q - 1)
+--       main_loop a''' i' j' p' q'
+--     else
+--       (a, i', j', p, q)
+
+--   let (final_arr, i_break, j_break, p_final, q_final) := main_loop arr' (left - 1) (right + 1) left right
+
+--   let rec move_left_eq (a : Vector α n) (k curr_j : Nat) : Vector α n × Nat :=
+--     if k > p_final then (a, curr_j)
+--     else
+--       let a' := a.swap k curr_j sorry sorry
+--       move_left_eq a' (k + 1) (curr_j - 1)
+
+--   let rec move_right_eq (a : Vector α n) (k curr_i : Nat) : Vector α n × Nat :=
+--     if k < q_final then (a, curr_i)
+--     else
+--       let a' := a.swap k curr_i sorry sorry
+--       move_right_eq a' (k - 1) (curr_i + 1)
+
+--   let (arr_l_done, lt_end) := move_left_eq final_arr left j_break
+--   let (arr_r_done, gt_start) := move_right_eq arr_l_done right i_break
+
+
+--   ⟨⟨arr_r_done, lt_end, gt_start⟩, by sorry, by sorry⟩
+-- #eval! Partition.bentleyMcIlroy #v[9,  3,  1,  8,  6,  2,  5,  0,  7,  4]  0 9 (by omega) (by omega)
